patch/PatchTheorems.lean
@@ -313,11 +313,11 @@ def HEqRefl {α : Sort u} (a : α) : HEq a a := HEq.refl a
 
 theorem nat_iota_zero {motive : Nat → Sort u} (zero : motive Nat.zero)
   (succ : (n : Nat) → (ih : motive n) → motive (n.succ)) :
-  Nat.rec (motive := motive) zero succ 0 = zero := rfl
+  Nat.rec (motive := motive) zero succ 0 ≍ zero := by rfl
 
 theorem nat_iota_succ {motive : Nat → Sort u} (zero : motive Nat.zero)
-  (succ : (n : Nat) → (ih : motive n) → motive (n.succ)) (t : Nat) :
-  Nat.rec (motive := motive) zero succ t.succ =
-  succ t (Nat.rec (motive := motive) zero succ t) := rfl
+  (succ : (n : Nat) → (ih : motive n) → motive n.succ) (t : Nat) :
+  Nat.rec (motive := motive) zero succ t.succ ≍
+  succ t (Nat.rec (motive := motive) zero succ t) := by rfl
 
 end L4L
